An initial draft of interpretation for STMonad.

theories/Monads/STMonad.v
@@ -62,34 +62,87 @@ From ITree Require Import
 .
 
 Import Monads.
-Import MonadNotation.
 Import ListNotations.
-From Coq Require Import
-     Morphisms
-     Setoid
-     Relation_Definitions
-     RelationClasses
+From Stdlib Require Import
+  Morphisms
+  Setoid
+  Relation_Definitions
+  RelationClasses
+  Arith.PeanoNat
+  Arith.Peano_dec
+  Init.Peano
 .
 Import ProperNotations.
 Local Open Scope monad_scope.
 Local Open Scope string_scope.
 
-(* Variant st : Type -> Type :=
- *   | MkST (T : Type) : st T.  *)
-
-Axiom STRef : forall (S A : Type), Type. 
-Axiom Idx : forall (S : Type), Type.
-
-Axiom IdxDecEq : forall (S : Type) (i1 i2 : Idx S),  
-    {i1 = i2} + {i1 <> i2}.
-
-Axiom STRefToIdx : forall (S A : Type) (ref : STRef S A),
-    Idx S.
 
 
-(* Variant STRef : Type -> Type -> Type :=
- *   | MkStRef (S : Type) (idx : nat) : STRef S nat. *)
+Module Type ST_SIG.
+
+  Parameter Idx : forall (S : Type), Type.
+  Parameter STRef : forall S A : Type, Type. 
+  Parameter IdxDecEq : forall (S : Type) (i1 i2 : Idx S),  
+      {i1 = i2} + {i1 <> i2}.
+  (* TODO: can we tie the result index to the stref here? *)
+  Parameter mkSTRef : forall S A : Type, Idx S -> STRef S A.
+  Parameter STRefToIdx : forall (S A : Type), STRef S A -> Idx S. 
+
+
+  (* Used to generate fresh, unique indices.*)
+  Parameter IdxGenE : Type -> Type.
+  Parameter newIdx :
+    forall {S : Type}
+      {E : Type -> Type} `{IdxGenE -< E}
+      , itree E (Idx S). 
+
+  (* TODO: better naming... *)
+  Parameter IdxRefSameIdx: forall (S A : Type) (idx : Idx S), (STRefToIdx S A (mkSTRef S A idx)) = idx.
+  Parameter IdxRefSameRef: forall (S A : Type) (ref : STRef S A), (mkSTRef S A (STRefToIdx S A ref)) = ref.
+
+
+End ST_SIG.
+
+Module ST_IMPL : ST_SIG.
+
+  Variant STRef' : Type -> Type -> Type :=
+    | MkStRef (S A : Type) (idx : nat) : STRef' S A.
+
+  Definition STRef := STRef'. 
+
+  Definition Idx (S : Type) := nat.
+
+
+  Definition mkSTRef := MkStRef.
+
+  Definition IdxDecEq (S : Type) (i1 i2 : Idx S)
+    : {i1 = i2} + {i1 <> i2} := Nat.eq_dec i1 i2.
+
+  Definition STRefToIdx (S A : Type) (ref : STRef' S A) : Idx S :=
+   match ref with
+   | MkStRef _ _ idx => idx
+   end. 
+
+  Inductive GenNum : Type -> Type :=
+  | NewNat : GenNum nat.
+
+  Definition IdxGenE := GenNum.
+
+  Definition newIdx {S : Type}
+    {E : Type -> Type} `{IdxGenE -< E} 
+    : itree E (Idx S) := trigger NewNat.
+
+
+  Lemma IdxRefSameIdx : forall (S A : Type) (idx : Idx S), (STRefToIdx S A (mkSTRef S A idx)) = idx.
+  Proof. intros. cbn. reflexivity. Qed.
+         
+  Lemma IdxRefSameRef : forall (S A : Type) (ref : STRef S A), (mkSTRef S A (STRefToIdx S A ref)) = ref.
+  Proof. intros. cbn. unfold STRefToIdx. destruct ref. reflexivity. Qed.
   
+
+End ST_IMPL.
+
+Import ST_IMPL.
 
 (* TODO: Expand to cover more types than nat *)
 Variant STEvent (S : Type) : Type -> Type :=
@@ -99,17 +152,7 @@ Variant STEvent (S : Type) : Type -> Type :=
 .
 
 
-(* TODO: make this typecheck *)
-
-
-
-(* TODO: Unfortunate duplication from tests/monadic/itree_effects/ITreeEffects.v*)
-Inductive randomE : Type -> Type :=
-| RandomNat : nat -> randomE nat.
-
-(* TODO: Drop 100000 bound here?*)
-Definition randomNat {E : Type -> Type} `{randomE -< E} : itree E nat :=
-  trigger (RandomNat 100). 
+(* Used for runtime checks, though an ideal impl won't need these. *)
 
 Variant Err : Type :=
 | Error (x : string) : Err.
@@ -117,14 +160,26 @@ Variant Err : Type :=
 Definition failwith
   {E : Type -> Type} `{exceptE Err -< E}
   {A:Type} (s:string) : itree E A := throw (Error s).
+  
 
 Section Translation.
 
   Context {E : Type -> Type}.
   Context {S : Type}.
   Context `{STEvent S -< E}. 
+
   
-  (* TODO: nit; switch to embed instead of trigger? *)
+  Definition lookup_err
+    {E : Type -> Type} {R : Type}
+    `{exceptE Err -< E}
+    {map} `{Map (Idx S) R map}
+    (k : (Idx S)) (mem : map) : itree E R :=
+    match lookup k mem with
+      | None => throw (Error "Failed to find key in map")
+      | Some v => Ret v
+    end.
+
+  
   Definition newSTRef (v : nat) : itree E (STRef S nat) :=
     trigger (NewSTRef S v). 
 
@@ -134,6 +189,19 @@ Section Translation.
   Definition writeSTRef (ref : STRef S nat) (a : nat) : itree E unit :=
     trigger (WriteSTRef S ref a).
 
+
+  Definition handle_STEvent
+    {map} `{Map (Idx S) nat map}
+    `{IdxGenE -< E} `{exceptE Err -< E}
+    : forall (T : Type),  STEvent S T -> stateT map (itree E) T :=
+    fun T e mem =>
+    match e in (STEvent _ T0) return (itree E (map * T0)) with
+    | NewSTRef _ v => idx <- newIdx;; Ret (add idx v mem, mkSTRef S nat idx)
+    | ReadSTRef _ s =>
+        let idx := STRefToIdx S nat s in v <- lookup_err idx mem;; Ret (mem, v)
+    | WriteSTRef _ s n => let idx := STRefToIdx S nat s in Ret (add idx n mem, tt)
+    end.
+
 End Translation.
 
 (* Example Programs*)
@@ -141,30 +209,36 @@ Section ExampleTrees.
 
   Context {S : Type}.
   Context {E : Type -> Type}.
-  Context `{randomE -< E}.
+  Context `{IdxGenE -< E}.
   Context `{exceptE Err -< E}.
 
 
   Definition E0 := STEvent S +' E.
 
-  Definition newAndReadBoth : itree (STEvent S) (nat * nat) :=
+  Definition newAndReadBoth : itree E0 (nat * nat) :=
     r1 <- newSTRef 5 ;;
     r2 <- newSTRef 6 ;;
     x1 <- readSTRef r1 ;;
     x2 <- readSTRef r2 ;;
     Ret (x1, x2).
 
-  (* NOTE: this should not work! *)
-  Fail Definition tree_escape_example : itree E0 nat :=
+  Definition tree_simp : itree E0 nat :=
     v <- newSTRef 5;;
-    writeSTRef v (match v with MkStRef _ idx => idx end);;
     readSTRef v.
 
-  Definition tree2 : itree E0 nat :=
+  (* NOTE: this failing definition is intentional, it should fail.
+    The intent is to test that we don't allow reference indices to escape. *)
+  Fail Definition tree_escape_example : itree E0 nat :=
+    v <- newSTRef 5;;
+    writeSTRef v (match v with mkSTRef _ _ idx => idx end);;
+    readSTRef v.
+
+  Definition tree_simp_another : itree E0 nat :=
     v <- newSTRef 5;;
     writeSTRef v 6;;
     val <- readSTRef v;;
-    ret val.
+    Ret val.
+
 
 End ExampleTrees.
 
@@ -174,8 +248,7 @@ End ExampleTrees.
 Section MemoryRep.
 
 Inductive node : Type := (* TODO: More types! *)
-  | NInt (x : nat) : node
-.
+  | NInt (x : nat) : node.
 
 
 Fixpoint node_to_type (n : node) : Type :=
@@ -190,70 +263,21 @@ Class Convertible t := {
     node_convert_inverse: forall v : t, (from_node (to_node v)) = Some v
   }.
 
+
 End MemoryRep.
 
 (* Interpretation in Rocq *)
 
 
-
 Section InterpST.
 
-  (* Context {E : Type -> Type}.
-   * Context {S : Type}. *)
-
-  Definition stStateT (s : Type) (m : Type -> Type) (a : Type) : Type :=
-    s -> m (prod s a).
-
-  Definition stState (s a : Type) := s -> prod s a.
-
-  Definition run_stStateT {s m a} (x : stStateT s m a) : s -> m (s * a)%type := x.
-
-  Definition lookup_err
-    {E : Type -> Type} `{exceptE Err -< E}
-    {map} `{Map nat nat map}
-    (k : nat) (mem : map) : itree E nat :=
-    match lookup k mem with
-      | None => throw (Error "Failed to find key in map")
-      | Some v => ret v
-    end.
 
 
-  (* TODO: Cleanup! *)
-  Definition handle_STEvent
-    {E : Type -> Type} {S : Type}
-    {map} `{Map nat nat map}
-    `{randomE -< E} `{exceptE Err -< E}
-    : forall (T : Type),  STEvent S T -> stateT map (itree E) T :=
-    fun T e mem =>
-    match e in (STEvent _ T0) return (itree E (map * T0)) with
-    | NewSTRef _ v =>
-        (fun v0 : nat => idx <- randomNat;; ret (add idx v0 mem, MkStRef S idx)) v
-    | ReadSTRef _ s =>
-        (fun s0 : STRef S nat =>
-        let S0 := nat in
-        match s0 in (STRef T0 T1) return (Map T1 T1 map -> itree E (map * T1)) with
-        | MkStRef S1 idx =>
-            (fun (_ : Type) (idx0 : nat) (H2 : Map nat nat map) =>
-              v <- lookup_err idx0 mem;; ret (mem, v)) S1 idx
-        end H) s
-    | WriteSTRef _ s n =>
-        (fun (s0 : STRef S nat) (n0 : nat) =>
-        let S0 := nat in
-        match
-          s0 in (STRef T0 T1) return (Map T1 T1 map -> T1 -> itree E (map * unit))
-        with
-        | MkStRef S1 idx =>
-            (fun (_ : Type) (idx0 : nat) (H2 : Map nat nat map) (n1 : nat) =>
-              ret (add idx0 n1 mem, tt)) S1 idx
-        end H n0) s n
-    end.
-
-  
   (* TODO: better name perhaps *)
   Definition handle_STEvent_leave_rest
-    {mem} `{Map nat nat mem}
-    {E : Type -> Type} {S : Type}
-    `{exceptE Err -< E} `{randomE -< E}
+    {S : Type}
+    {mem} `{Map (Idx S) nat mem}
+    {E : Type -> Type} `{exceptE Err -< E} `{IdxGenE -< E}
     (T : Type) (e : (STEvent S +' E) T)
     : stateT mem (itree (E)) T :=
     match e with
@@ -262,20 +286,54 @@ Section InterpST.
     end.
 
 
+  Global Instance reldec_idx {S : Type} : @RelDec.RelDec (Idx S) eq :=
+    (RelDec.RelDec_from_dec eq (IdxDecEq S)).
+    
+  Global Instance map_from_idx {S : Type} {V : Type}  : 
+    Map (Idx S) V (alist (Idx S) V) :=
+    Map_alist (RelDec.RelDec_from_dec eq (IdxDecEq S)) V.
+
+  Global Instance reldec_idx_correct {S : Type} : @RelDec.RelDec_Correct (Idx S) eq reldec_idx.
+  econstructor.
+  intuition.
+  destruct (IdxDecEq S x y); try assumption.
+  - unfold RelDec.rel_dec in H. cbn in H.
+    destruct IdxDecEq in H.
+    + contradiction.
+    + discriminate H.
+  - cbn.
+    specialize (@reldec_idx S) as reldec.
+    specialize (IdxDecEq S x y) as dec.
+    destruct dec.
+    + unfold RelDec.rel_dec. unfold reldec_idx. unfold RelDec.RelDec_from_dec.
+      destruct (IdxDecEq S x y).
+      * reflexivity.
+      * contradiction.
+    + contradiction.
+    Qed.
+
+
+  Global Instance map_idx_correct {S V : Type} :
+    MapOk eq (@map_from_idx S V).
+  unfold map_from_idx.
+  eapply MapLaws_alist; typeclasses eauto.
+  Qed.
+
   Definition interp_st
     {E : Type -> Type} {S : Type}
-    `{exceptE Err -< E} `{randomE -< E}
-    {mem} `{Map nat nat mem}
+    `{exceptE Err -< E} `{IdxGenE -< E}
+    {mem} `{Map (Idx S) nat mem}
     : itree (STEvent S +' E) ~> stateT mem (itree (E)) :=
     interp_state handle_STEvent_leave_rest.
 
   
+  (* TODO: cleanup! *)
+  (* TODO: refactor to use interp_map? *)
   Definition runSt {A : Type} {E : Type -> Type}
-    {map} `{Map nat nat map} `{exceptE Err -< E} `{randomE -< E}
-    : (forall (S : Type), itree ((STEvent S) +' E) A) -> itree E A :=
-  fun f =>
-  let tree := f unit in
-  fmap snd (interp_st _ tree Maps.empty).
+     `{exceptE Err -< E} `{IdxGenE -< E}
+    (f : forall (S : Type), itree ((STEvent S) +' E) A)
+    : itree E A :=
+    fmap snd (interp_st _ (f unit) Maps.empty).
 
   
   
@@ -287,18 +345,22 @@ End InterpST.
 Section InterpSTTheorems.
 
   (* TODO: refactor to above. *)
-  (* Context {E : Type -> Type}.
-   * Context `{exceptE Err -< E}.
-   * Context `{randomE -< E}. *)
+  Context {E : Type -> Type}. (* other events *)
+  Context {S : Type}. (* state thread *)
+  Context `{exceptE Err -< E}. (* runtime checks  *)
+  Context `{IdxGenE -< E}. (* index generating event *)
+  Context {R : Type}. (* values contained in the map,  TODO: expand from one value type. *)
 
-  Definition mem := alist nat nat.
+  Definition mem := alist (Idx S) nat. 
+  Global Instance mem_instance {V : Type} : 
+    Map (Idx S) V (alist (Idx S) V) :=
+    Map_alist (RelDec.RelDec_from_dec eq (IdxDecEq S)) V.
 
 
-  Definition _interp_st {R E S}
-    `{exceptE Err -< E} `{randomE -< E}
-    (ot : itree' (STEvent S +' E) R)
+  Definition _interp_st {T : Type}
+    (ot : itree' (STEvent S +' E) T)
     (l : mem)
-    : itree (E) (mem * R) :=
+    : itree E (mem * T) :=
     match ot with
     | RetF r => ret (l, r)
     | TauF t => Tau (interp_st _ t l)
@@ -307,15 +369,13 @@ Section InterpSTTheorems.
         Tau (interp_st _ (k (snd x)) (fst x))
     end.
 
-
-  Lemma unfold_interp_st {R E} {S : Type}
-    `{exceptE Err -< E} `{randomE -< E}
-    (t : itree (STEvent S +' E) R)
+  Lemma unfold_interp_st {T : Type}
+    (t : itree (STEvent S +' E) T)
     (l : mem) :
     eq_itree eq
     (interp_st _ t l)
     (_interp_st (observe t) l).
-  Proof.
+  Proof using Type.
     unfold interp_st, interp_state, interp, Basics.iter, MonadIter_stateT0, Basics.iter.
     cbn.
     setoid_rewrite unfold_iter; cbn.
@@ -330,56 +390,55 @@ Section InterpSTTheorems.
       reflexivity.
   Qed.
 
-  Lemma interp_st_ret: forall {R E S} `{exceptE Err -< E} `{randomE -< E} (val: R) (l : mem),
+  Lemma interp_st_ret: forall (val: R) (l : mem),
       @interp_st E S _ _ _ _ _ (ret val) l ≅ ret (l, val).
-    Proof.
+    Proof using Type.
       intros. rewrite unfold_interp_st. reflexivity.
     Qed.
 
-  Lemma interp_st_Ret: forall {R E S} `{exceptE Err -< E} `{randomE -< E} (val: R) (l : mem),
+  Lemma interp_st_Ret: forall (val: R) (l : mem),
       @interp_st E S _ _ _ _ _ (Ret val) l ≅ Ret (l, val).
-    Proof.
+    Proof using Type.
       intros. rewrite unfold_interp_st. reflexivity.
     Qed.
 
-  Lemma interp_st_Ret_eutt: forall {R E S} `{exceptE Err -< E} `{randomE -< E} (val: R) (l : mem),
+  Lemma interp_st_Ret_eutt: forall {T : Type} (val: T) (l : mem),
       @interp_st E S _ _ _ _ _ (Ret val) l ≈ Ret (l, val).
-    Proof.
+    Proof using Type.
       intros. rewrite unfold_interp_st. reflexivity.
     Qed.
 
   Lemma interp_st_vis
-    {T U E S} `{exceptE Err -< E} `{randomE -< E}
+    {T U} 
     (e : (STEvent S +' E) T)
     (k : T -> itree (STEvent S +' E) U)
     (l : mem)
     : interp_st _ (Vis e k) l
     ≅ x <- handle_STEvent_leave_rest _ e l;;
       Tau (interp_st _ (k (snd x)) (fst x)).
-    Proof.
+    Proof using Type.
       intros. rewrite unfold_interp_st. reflexivity.
     Qed.
 
     
-  Lemma interp_st_tau
-      {R E S} `{exceptE Err -< E} `{randomE -< E}
-      (t : itree (STEvent S +' E) R)
+  Lemma interp_st_tau {T : Type}
+      (t : itree (STEvent S +' E) T)
       (l : mem)
       : interp_st _ (Tau t) l ≅ Tau (interp_st _ t l).
-    Proof.
+    Proof using Type.
       intros. rewrite unfold_interp_st. reflexivity.
     Qed.
 
 
-  Lemma Ret_is_ret {E R} (x : R) : ((Ret x) : itree E R)  = ret x.
-    Proof. reflexivity. Qed.
+  Lemma Ret_is_ret (x : R) : ((Ret x) : itree E R)  = ret x.
+    Proof using Type. reflexivity. Qed.
     
   Lemma interp_st_trigger
-    {T E S} `{exceptE Err -< E} `{randomE -< E}
+    {T : Type} 
     (e : (STEvent S +' E) T)
     (l : mem) :
     interp_st _ (ITree.trigger e) l ≈ handle_STEvent_leave_rest _ e l.
-    Proof.
+    Proof using Type.
       unfold ITree.trigger.
       rewrite interp_st_vis.
       match goal with
@@ -397,10 +456,10 @@ Definition eq_itree_eqv_global {R E} (x1 x2 : itree (E) (mem * R)) : Prop :=
   @eq_itree (E) _ _ eq x1 x2.
 
 
-Global Instance eq_itree_interp_st {R E S} `{exceptE Err -< E} `{randomE -< E}: 
-Proper (@eq_itree (STEvent S +' E) R R eq ==> eq ==> eq_itree_eqv_global)
-        (interp_st R).
-Proof.
+Global Instance eq_itree_interp_st {T : Type} : 
+Proper (@eq_itree (STEvent S +' E) T T eq ==> eq ==> eq_itree_eqv_global)
+        (interp_st T).
+Proof using Type.
   repeat red.
   ginit. pcofix CIH. intros.
   rewrite !unfold_interp_st. punfold H2. red in H2.
@@ -414,61 +473,352 @@ Proof.
   Qed.
 
     
-  Lemma interp_st_bind {R U E S} `{exceptE Err -< E} `{randomE -< E}
-    (t : itree (STEvent S +' E) R)
-    (k : R -> itree (STEvent S +' E) U)
-    (mem : mem)
-    : interp_st U (bind t k) mem
-        ≅ '(new_mem, new_val) <- interp_st R t mem;;
-      interp_st U (k new_val) new_mem.
-    revert t k mem.
-    ginit. pcofix CIH.
-    intros t k mem.
-    assert (unfold_bind' : interp_st U (ITree.bind t k) mem
-                          ≅ interp_st U (bind_ t k) mem).
-    { apply eq_itree_interp_st. apply unfold_bind. reflexivity.  }
-    rewrite unfold_bind'.
-    rewrite (unfold_interp_st t mem).
-    destruct (observe t).
-    - cbn. rewrite !bind_ret_l. cbn. apply reflexivity.
-    - rewrite interp_st_tau. cbn. rewrite bind_tau.
-      gstep. econstructor; eauto with paco.
-    - rewrite interp_st_vis. cbn. rewrite bind_bind.
-      guclo eqit_clo_bind. econstructor.
-      + reflexivity.
-      + intros u2 ? []. destruct u2 eqn:Equ2.
-        rewrite bind_tau.
-        gstep. constructor.
-        auto with paco.
-  Qed.
+Lemma interp_st_bind {U} 
+  (t : itree (STEvent S +' E) R)
+  (k : R -> itree (STEvent S +' E) U)
+  (mem : mem)
+  : interp_st U (ITree.bind t k) mem
+      ≅ '(new_mem, new_val) <- interp_st R t mem;;
+    interp_st U (k new_val) new_mem.
+  revert t k mem.
+  ginit. pcofix CIH.
+  intros t k mem.
+  assert (unfold_bind' : interp_st U (ITree.bind t k) mem
+                        ≅ interp_st U (bind_ t k) mem).
+  { apply eq_itree_interp_st. apply unfold_bind. reflexivity.  }
+  rewrite unfold_bind'.
+  rewrite (unfold_interp_st t mem).
+  destruct (observe t).
+  - cbn. rewrite !bind_ret_l. cbn. apply reflexivity.
+  - rewrite interp_st_tau. cbn. rewrite bind_tau.
+    gstep. econstructor; eauto with paco.
+  - rewrite interp_st_vis. cbn. rewrite bind_bind.
+    guclo eqit_clo_bind. econstructor.
+    + reflexivity.
+    + intros u2 ? []. destruct u2 eqn:Equ2.
+      rewrite bind_tau.
+      gstep. constructor.
+      auto with paco.
+Qed.
 
+Lemma interp_st_bind_eutt {U} 
+  (t : itree (STEvent S +' E) R)
+  (k : R -> itree (STEvent S +' E) U)
+  (mem : mem)
+  : interp_st U (ITree.bind t k) mem
+      ≈ '(new_mem, new_val) <- interp_st R t mem;;
+    interp_st U (k new_val) new_mem.
+  revert t k mem.
+  ginit. pcofix CIH.
+  intros t k mem.
+  assert (unfold_bind' : interp_st U (ITree.bind t k) mem
+                        ≅ interp_st U (bind_ t k) mem).
+  { apply eq_itree_interp_st. apply unfold_bind. reflexivity.  }
+  rewrite unfold_bind'.
+  rewrite (unfold_interp_st t mem).
+  destruct (observe t).
+  - cbn. rewrite !bind_ret_l. cbn. apply reflexivity.
+  - rewrite interp_st_tau. cbn. rewrite bind_tau.
+    gstep. econstructor; eauto with paco.
+  - rewrite interp_st_vis. cbn. rewrite bind_bind.
+    guclo eqit_clo_bind. econstructor.
+    + reflexivity.
+    + intros u2 ? []. destruct u2 eqn:Equ2.
+      rewrite bind_tau.
+      gstep. constructor.
+      auto with paco.
+Qed.
+
+Lemma interp_st_bind_eutt' {U} 
+  (t : itree (STEvent S +' E) R)
+  (k : R -> itree (STEvent S +' E) U)
+  (mem : mem)
+  : (interp_st U (ITree.bind t k) mem)
+      ≈ '(new_mem, new_val) <- interp_st R t mem;;
+    interp_st U (k new_val) new_mem.
+  revert t k mem.
+  ginit. pcofix CIH.
+  intros t k mem.
+  assert (unfold_bind' : interp_st U (ITree.bind t k) mem
+                        ≅ interp_st U (bind_ t k) mem).
+  { apply eq_itree_interp_st. apply unfold_bind. reflexivity.  }
+  rewrite unfold_bind'.
+  rewrite (unfold_interp_st t mem).
+  destruct (observe t).
+  - cbn. rewrite !bind_ret_l. cbn. apply reflexivity.
+  - rewrite interp_st_tau. cbn. rewrite bind_tau.
+    gstep. econstructor; eauto with paco.
+  - rewrite interp_st_vis. cbn. rewrite bind_bind.
+    guclo eqit_clo_bind. econstructor.
+    + reflexivity.
+    + intros u2 ? []. destruct u2 eqn:Equ2.
+      rewrite bind_tau.
+      gstep. constructor.
+      auto with paco.
+Qed.
+
+
+Lemma eutt_eq_bind_interp_st {U}
+  (k2 : (mem * R) -> itree E (mem * U))
+  (lmem : mem)
+  (t1 : itree (STEvent S +' E) R)
+  (t2 : itree E (mem * R))
+  (k1: R -> itree (STEvent S +' E) U)
+  :
+  interp_st R t1 lmem ≈ t2 ->
+  (forall u lmem', interp_st U (k1 u) lmem' ≈ (k2 (lmem', u))) ->
+  interp_st U (ITree.bind t1 k1) lmem
+  ≈
+  ITree.bind t2 k2.
+Proof.
+  intros t1_eq keq.
+  rewrite (interp_st_bind_eutt t1 k1).                                                                                
+  apply eutt_eq_bind'; [assumption | intuition].
+Qed.
 
 End InterpSTTheorems.
 
+
+Section STLookupErr.
+
+  Context {E : Type -> Type}.
+  Context {S : Type}.
+  Context `{exceptE Err -< E}.
+  Context {R : Type}.
+  Context {map : Type}.
+  Context {Map : Map (Idx S) R map}.
+  Context {MOK : MapOk eq Map}.
+
+  Lemma st_lookup_err_add_eq : forall (s : map) (k : Idx S) (v : R),
+      lookup_err k (Maps.add k v s) = @ret (itree E) _ _ v.
+  Proof using MOK.
+    intros. unfold lookup_err.
+    rewrite (@lookup_add_eq (Idx S) R map Map MOK).
+    reflexivity.
+  Qed.
+
+  Lemma st_lookup_err_remove_eq : forall (k : Idx S) (s : map),
+      lookup_err k (Maps.remove k s) = @throw Err E _ _ (Error "Failed to find key in map").
+  Proof using MOK.
+    intros. unfold lookup_err.
+    rewrite (@lookup_remove_eq (Idx S) R map Map MOK k s).
+    reflexivity.
+  Qed.
+
+End STLookupErr.
+
+
+
 Require Stdlib.derive.Derive.
+Section Examples.
 
-Section Example1.
-  
-  Definition E1 :=
-  Derive tree1_simplified SuchThat
-    ( runSt (fun S => @tree1 S E0)
-        ≈
-      tree1_simplified 
-    ) As tree_simplification_works.
+  Context {S : Type}.
+  Context {E : Type -> Type}.
+  Context `{IdxGenE -< E}.
+  Context `{exceptE Err -< E}.
 
+  Lemma eutt_fmap {E' : Type -> Type} {R U : Type} {t1 t2 : itree E' R} {f : R -> U} :
+    t1 ≈ t2 ->
+    fmap f t1 ≈ fmap f t2.
+    Proof using Type.
+      intros t_eq. apply eqit_map with (RR := eq).
+      + intros.
+        f_equal. assumption.
+      + apply t_eq.
+    Qed.
 
-End Example1.
-  
-Derive (out_tree : itree E) in (
+       
     
-  )  
-Example ex1_run {E : Type -> Type} `{exceptE Err -< E} `{randomE -< E} :
-  runSt (fun S => @tree1 S E) = runSt (fun S => tree1).
-unfold runSt at 1.
-unfold tree1. 
-Fail setoid_rewrite interp_st_bind. (* TODO: fix this! *)
-  
+  Lemma eutt_eq_bind {U R} (t : itree E U) (k1 k2: U -> itree E R):
+    (forall u, (k1 u) ≈ (k2 u)) ->
+    (ITree.bind t k1) ≈ (ITree.bind t k2).
+  Proof using Type. apply eutt_eq_bind. Qed.
+    
 
+  Lemma eutt_eq_bind' {U R}
+    (k1 k2: U -> itree E R)
+    (t1 t2: itree E U):
+    t1 ≈ t2 ->
+    (forall u, (k1 u) ≈ (k2 u)) ->
+    (ITree.bind t1 k1) ≈ (ITree.bind t2 k2).
+  Proof. apply eutt_eq_bind'. Qed.
+
+(* TODO: move to separate ltac section. *)
+Ltac refine_prod :=
+  (refine (fun '(a,b) => _)).
+
+Ltac refine_arg :=
+  (refine (fun arg => _)).
+
+Ltac refine_arg2 :=
+  (refine (fun arg1 arg2 => _)).
+
+
+
+Theorem bind_Ret_l : forall A B (f : A -> itree E B) (x : A), bind (Ret x) f ≈ f x.
+  setoid_rewrite Ret_is_ret.
+  setoid_rewrite Monad.bind_ret_l.
+  reflexivity.
+  Qed.
+          
+
+Theorem bind_Ret_r : forall A (x : itree E A), bind x (fun y => Ret y) ≈ x.
+  intros A x. setoid_rewrite Monad.bind_ret_r. reflexivity. Qed.
+
+
+Ltac monad_simpl_inner :=
+  repeat (repeat setoid_rewrite Monad.bind_bind;
+          repeat setoid_rewrite bind_Ret_l;
+          repeat setoid_rewrite bind_Ret_r).
+
+
+
+(* Useful for lifting ITree's back to a monad instance. *)
+Ltac change_to_monad :=
+  change (@ITree.bind ?E) with (@Monad.bind (itree E) _);
+  try setoid_rewrite Ret_is_ret.
+
+Ltac bind_split_refl_intros split_tactic :=
+  split_tactic ;[ reflexivity | intros]
+  ;cbv beta match.
+
+Opaque Maps.add.
   
+  Derive (tree_simplified : itree E nat) in
+    ( runSt (fun S => @tree_simp S E)
+        ≈
+      tree_simplified
+    ) as tree_simplification.
+  Proof.
+    etransitivity.
+    { unfold runSt.
+      eapply eutt_fmap.
+      eapply (eutt_eq_bind_interp_st ltac:(refine_prod)).
+      - unfold newSTRef.
+        rewrite interp_st_trigger.
+        cbn.
+        reflexivity.
+      - intros u lmem'.
+        unfold readSTRef.
+        rewrite interp_st_trigger.
+        cbn.
+        reflexivity. }
+    etransitivity.
+    { eapply eutt_fmap.
+      change_to_monad.
+      monad_simpl_inner.
+      bind_split_refl_intros ltac:(eapply (eutt_eq_bind' _ ltac:(refine_arg))).
+      rewrite IdxRefSameIdx.
+      rewrite st_lookup_err_add_eq.
+      monad_simpl_inner.
+      reflexivity. }
+    cbn.
+    setoid_rewrite map_bind.
+    setoid_rewrite map_ret.
+    unfold snd.
+    unfold tree_simplified.
+    reflexivity.
+  Defined.
+
+
+  (* TODO: fill out the other examples in a likewise manner to above. *)
+  Derive (readboth_simplified : itree E (nat*nat)) in
+    ( runSt (fun S => @newAndReadBoth S E)
+        ≈
+      readboth_simplified
+    ) as tree_simplification2.
+  Proof.
+    etransitivity.
+    { unfold runSt.
+      eapply eutt_fmap.
+      eapply (eutt_eq_bind_interp_st ltac:(refine_arg)).
+      - unfold newSTRef.
+        rewrite interp_st_trigger.
+        cbn.
+        reflexivity.
+      - intros u lmem'.
+        unfold readSTRef.
+        eapply (eutt_eq_bind_interp_st ltac:(refine_arg)).
+        {
+          unfold newSTRef.
+          rewrite interp_st_trigger.
+          cbn.
+          change lmem' with (fst (lmem', u)). (* TODO: unfortunate change. *)
+          reflexivity.
+        }
+        intros ? ?.
+        eapply (eutt_eq_bind_interp_st ltac:(refine_arg)).
+        {
+          unfold newSTRef.
+          rewrite interp_st_trigger.
+          cbn. change u with (snd (lmem', u)).
+          change lmem'0 with (fst (lmem'0, u0)).
+          reflexivity.
+        }
+        intros ? ?. 
+        eapply (eutt_eq_bind_interp_st ltac:(refine_arg)).
+        {
+          unfold newSTRef.
+          rewrite interp_st_trigger.
+          cbn. change u with (snd (lmem', u)).
+          change lmem'0 with (fst (lmem'0, u0)).
+          change u0 with (snd (lmem'0, u0)).
+          change lmem'1 with (fst (lmem'1, u1)).
+          reflexivity.
+        }
+        intros ? ?.
+        rewrite interp_st_Ret.
+        change lmem'2 with (fst (lmem'2, u2)).
+        change u1 with (snd (lmem'1, u1)).
+        change u2 with (snd (lmem'2, u2)).
+        reflexivity. }
+    etransitivity.
+    { eapply eutt_fmap.
+      change_to_monad.
+      monad_simpl_inner.
+      bind_split_refl_intros ltac:(eapply (eutt_eq_bind' _ ltac:(refine_arg))).
+      monad_simpl_inner.
+      bind_split_refl_intros ltac:(eapply (eutt_eq_bind' _ ltac:(refine_arg))).
+      monad_simpl_inner. cbn.
+      rewrite IdxRefSameIdx.
+      Transparent Maps.add. unfold lookup_err at 1.
+      assert (lookup u (add u0 6 (add u 5 [])) = Some 5).
+      {
+        cbn. give_up. (* TODO: needs uniqueness of elements from stream. *)
+      }
+
+      setoid_rewrite H1.
+      monad_simpl_inner.
+      setoid_rewrite IdxRefSameIdx.
+      setoid_rewrite st_lookup_err_add_eq.
+      monad_simpl_inner.
+      reflexivity.
+    }
+    cbn.
+    setoid_rewrite map_bind.
+    setoid_rewrite map_bind.
+    setoid_rewrite map_ret.
+    unfold snd.
+    unfold readboth_simplified.
+    reflexivity.
+    Abort.
+
+End Examples.
 
 (* CPP Bindings *)
+
+  
+From Crane Require Extraction.
+
+
+(* TODO: how to obtain integer reference statically? *)
+Crane Extract Inlined Constant STRef => "%t1".
+Crane Extract Inlined Constant newSTRef => "%result = %a0".
+Crane Extract Inlined Constant readSTRef => "%a0". 
+Crane Extract Inlined Constant writeSTRef => "%a0 = %a1".
+Crane Extract Skip IdxRefSameIdx.
+Crane Extract Skip IdxRefSameRef.
+Crane Extract Skip E0.
+Crane Extract Skip newIdx.
+
+
